theories/SmallStep/All.v
@@ -3,3 +3,4 @@ Require Export theories.SmallStep.Typing.All.
 Require Export theories.SmallStep.Runtime.All.
 Require Export theories.SmallStep.Soundness.All.
 Require Export theories.SmallStep.Determinism.All.
+Require Export theories.SmallStep.Public.
