theories/SmallStep/Determinism/All.v
@@ -1,2 +1,3 @@
 Require Export theories.SmallStep.Determinism.Terminal.
-Require Export theories.SmallStep.Determinism.Scheduler.
+Require Export theories.SmallStep.Determinism.SchedulerPrelude.
+Require Export theories.SmallStep.Determinism.SchedulerPublic.
